prove ELI spec for Spinlock lock fun

src/example/SpinlockSpec1.v
@@ -24,18 +24,17 @@ Section SPEC.
   Context {TLRAS : TLRAs STT Γ Σ}.
 
   Context {HasMEMRA: @GRA.inG memRA Γ}.
-  Context {HasOneShots : @GRA.inG (OneShots.t unit) Γ}.
-  Context {HasAuthExcls1 : @GRA.inG (AuthExcls.t (nat * nat)) Γ}.
-  Context {HasAuthExcls2 : @GRA.inG (AuthExcls.t nat) Γ}.
+  (* Context {HasOneShots : @GRA.inG (OneShots.t unit) Γ}. *)
+  (* Context {HasAuthExcls1 : @GRA.inG (AuthExcls.t (nat * nat)) Γ}. *)
+  Context {HasAuthExcls : @GRA.inG (AuthExcls.t nat) Γ}.
 
-  Ltac red_tl_all := red_tl; red_tl_memra; red_tl_oneshots; red_tl_authexcls.
+  Ltac red_tl_all := red_tl; red_tl_memra; red_tl_authexcls.
+  (* Ltac red_tl_all := red_tl; red_tl_memra; red_tl_oneshots; red_tl_authexcls. *)
 
   (** Invariants. *)
-  Definition spinlockInv (n : nat) (x : SCMem.val) (γx : nat) (P : sProp n)
+  Definition spinlockInv (n : nat) (x : SCMem.val) (γx : nat) (S : sProp n)
     : sProp n :=
-    (((x ↦ 0) ∗ (● γx 0) ∗ P)
-     ∨ ((x ↦ 1) ∗ (● γx 1))
-    )%S.
+    (∃ (s : τ{nat}), (x ↦ s) ∗ (● γx s) ∗ ((⌜s = 0⌝ ∗ S) ∨ (⌜s = 1⌝)))%S.
 
   (* Definition spinlockInv (n : nat) (γ : nat) (x : SCMem.val) (P : sProp n) (k l : nat) *)
   (*   : sProp n := *)
@@ -56,15 +55,16 @@ Section SPEC.
 
   (* Namespace for Spinlock invariants. *)
   Definition N_Spinlock1 : namespace := (nroot .@ "Spinlock1").
+  Notation E_Spinlock1 := (↑N_Spinlock1 : coPset).
 
-  Definition isSpinlock n (γ : nat) (x : SCMem.val) (P : sProp n) (k L l : nat)
+  Definition isSpinlock n (x : SCMem.val) (γx : nat) (S : sProp n) (k L : nat)
     : sProp n :=
     (∃ (N : τ{namespace, n}),
         (⌜(↑N ⊆ (↑N_Spinlock1 : coPset))⌝)
-          ∗ ◆[k, L] ∗ (⌜0 < l⌝) ∗ syn_inv n N (spinlockInv n γ x P k l))%S.
+          ∗ ◆[k, L] ∗ syn_inv n N (spinlockInv n x γx S))%S.
 
-  Global Instance isSpinlock_persistent n γ x P k L l :
-    Persistent (⟦isSpinlock n γ x P k L l, n⟧).
+  Global Instance isSpinlock_persistent n x γx S k L :
+    Persistent (⟦isSpinlock n x γx S k L, n⟧).
   Proof.
     unfold Persistent. iIntros "H". unfold isSpinlock. red_tl.
     iDestruct "H" as "[%N H]". iExists N. red_tl. rewrite red_syn_inv.
@@ -74,415 +74,268 @@ Section SPEC.
   (* Lemma mask_disjoint_spinlock_state_tgt : ↑N_Spinlock1 ## (↑N_state_tgt : coPset). *)
   (* Proof. apply ndot_ne_disjoint. ss. Qed. *)
 
-  Lemma make_isSpinlock
-        n γ x P γk k L l (LT : 0 < l)
-        (q : Qp) (γu u : nat) Es
-    :
-    ⊢
-      ⟦((x ↦ 0) ∗ ➢(auexa_b γ (q, γu, u)) ∗ ➢(auexa_w γ (q, γu, u)) ∗ (⤉P) ∗ ◆[k, L] ∗ ◇[k](1+l, 1))%S, 1+n⟧
-        -∗
-        ⟦( =|1+n|={Es}=> (⤉(isSpinlock n γ x P γk k L l)))%S, 1+n⟧.
-  Proof.
-    red_tl. simpl. iIntros "(PT & BQ & WQ & P & #LO & PC)".
-    rewrite red_syn_fupd. red_tl.
-    iMod ((FUpd_alloc _ _ _ n (↑(N_Spinlock.@"a")) (spinlockInv n γ x P γk k l))
-           with "[PT BQ WQ P PC]") as "#SINV".
-    auto.
-    { simpl. unfold spinlockInv. red_tl. iLeft. iExists q. red_tl. iExists γu. red_tl. iExists u.
-      red_tl. iSplitL "BQ". iFrame. iLeft. iFrame.
-    }
-    iModIntro. unfold isSpinlock. red_tl.
-    iExists (↑(N_Spinlock.@"a")). red_tl. iSplit.
-    { iPureIntro. apply nclose_subseteq. }
-    simpl. rewrite red_syn_inv. auto.
-  Qed.
+  (* Lemma make_isSpinlock *)
+  (*       n γ x P γk k L l (LT : 0 < l) *)
+  (*       (q : Qp) (γu u : nat) Es *)
+  (*   : *)
+  (*   ⊢ *)
+  (*     ⟦((x ↦ 0) ∗ ➢(auexa_b γ (q, γu, u)) ∗ ➢(auexa_w γ (q, γu, u)) ∗ (⤉P) ∗ ◆[k, L] ∗ ◇[k](1+l, 1))%S, 1+n⟧ *)
+  (*       -∗ *)
+  (*       ⟦( =|1+n|={Es}=> (⤉(isSpinlock n γ x P γk k L l)))%S, 1+n⟧. *)
+  (* Proof. *)
+  (*   red_tl. simpl. iIntros "(PT & BQ & WQ & P & #LO & PC)". *)
+  (*   rewrite red_syn_fupd. red_tl. *)
+  (*   iMod ((FUpd_alloc _ _ _ n (↑(N_Spinlock.@"a")) (spinlockInv n γ x P γk k l)) *)
+  (*          with "[PT BQ WQ P PC]") as "#SINV". *)
+  (*   auto. *)
+  (*   { simpl. unfold spinlockInv. red_tl. iLeft. iExists q. red_tl. iExists γu. red_tl. iExists u. *)
+  (*     red_tl. iSplitL "BQ". iFrame. iLeft. iFrame. *)
+  (*   } *)
+  (*   iModIntro. unfold isSpinlock. red_tl. *)
+  (*   iExists (↑(N_Spinlock.@"a")). red_tl. iSplit. *)
+  (*   { iPureIntro. apply nclose_subseteq. } *)
+  (*   simpl. rewrite red_syn_inv. auto. *)
+  (* Qed. *)
 
-  Lemma init_isSpinlock
-        n x P γk k L l (LT : 0 < l)
-        Es
-    :
-    ⊢
-      ⟦(➢(auexa) ∗ (x ↦ 0) ∗ (⤉P) ∗ ◆[k, L] ∗ ◇[k](1+l, 1))%S, 1+n⟧
-        -∗
-        ⟦( =|1+n|={Es}=> (➢(auexa) ∗ ∃ (γ : τ{nat}), ⤉(isSpinlock n γ x P γk k L l)))%S, 1+n⟧.
-  Proof.
-    red_tl. simpl. iIntros "(AEA & PT & P & #LO & PC)".
-    rewrite red_syn_fupd. red_tl.
-    iMod (auexa_alloc_gt _ ((1%Qp, 0, 0)) with "AEA") as "[AEA (%γ & BQ & BW)]".
-    iPoseProof (make_isSpinlock n γ x P γk k L l with "[PT BQ BW P PC]") as "ISL".
-    auto.
-    { red_tl. iFrame. iApply "LO". }
-    iEval (rewrite red_syn_fupd) in "ISL". iMod "ISL".
-    iModIntro. iSplitL "AEA". iFrame. iExists γ. iFrame.
-  Qed.
+  (* Lemma init_isSpinlock *)
+  (*       n x P γk k L l (LT : 0 < l) *)
+  (*       Es *)
+  (*   : *)
+  (*   ⊢ *)
+  (*     ⟦(➢(auexa) ∗ (x ↦ 0) ∗ (⤉P) ∗ ◆[k, L] ∗ ◇[k](1+l, 1))%S, 1+n⟧ *)
+  (*       -∗ *)
+  (*       ⟦( =|1+n|={Es}=> (➢(auexa) ∗ ∃ (γ : τ{nat}), ⤉(isSpinlock n γ x P γk k L l)))%S, 1+n⟧. *)
+  (* Proof. *)
+  (*   red_tl. simpl. iIntros "(AEA & PT & P & #LO & PC)". *)
+  (*   rewrite red_syn_fupd. red_tl. *)
+  (*   iMod (auexa_alloc_gt _ ((1%Qp, 0, 0)) with "AEA") as "[AEA (%γ & BQ & BW)]". *)
+  (*   iPoseProof (make_isSpinlock n γ x P γk k L l with "[PT BQ BW P PC]") as "ISL". *)
+  (*   auto. *)
+  (*   { red_tl. iFrame. iApply "LO". } *)
+  (*   iEval (rewrite red_syn_fupd) in "ISL". iMod "ISL". *)
+  (*   iModIntro. iSplitL "AEA". iFrame. iExists γ. iFrame. *)
+  (* Qed. *)
 
-  Lemma update_isSpinlock
-        n γ x P γk k L l
-        Es
-        (MASK_SL : mask_has_Spinlock Es n)
-        γk' k' L' l' (LT' : 0 < l')
-    :
-    ⊢ ⟦((⤉(isSpinlock n γ x P γk k L l)) ∗ ➢(live γk k 1) ∗ ◆[k', L'] ∗ ◇[k'](1+ l', 1))%S, 1+n⟧
-       -∗
-       ⟦( =|1+n|={Es}=>((⤉ isSpinlock n γ x P γk' k' L' l') ∗ ➢(dead γk k)))%S, 1+n⟧.
+  (* Lemma update_isSpinlock *)
+  (*       n γ x P γk k L l *)
+  (*       Es *)
+  (*       (MASK_SL : mask_has_Spinlock Es n) *)
+  (*       γk' k' L' l' (LT' : 0 < l') *)
+  (*   : *)
+  (*   ⊢ ⟦((⤉(isSpinlock n γ x P γk k L l)) ∗ ➢(live γk k 1) ∗ ◆[k', L'] ∗ ◇[k'](1+ l', 1))%S, 1+n⟧ *)
+  (*      -∗ *)
+  (*      ⟦( =|1+n|={Es}=>((⤉ isSpinlock n γ x P γk' k' L' l') ∗ ➢(dead γk k)))%S, 1+n⟧. *)
+  (* Proof. *)
+  (*   red_tl. simpl. iIntros "(ISL & LIVE & LO' & PC')". rewrite red_syn_fupd. red_tl. *)
+  (*   iEval (unfold isSpinlock) in "ISL". red_tl. *)
+  (*   iDestruct "ISL" as "[%N ISL]". iEval red_tl in "ISL". *)
+  (*   iDestruct "ISL" as "(%IN & _ & %LT & SI)". rewrite red_syn_inv. *)
+  (*   iInv "SI" as "SI" "K". *)
+  (*   { unfold mask_has_Spinlock in MASK_SL. des_ifs. set_solver. } *)
+  (*   simpl. iEval (unfold spinlockInv; red_tl) in "SI". *)
+  (*   iDestruct "SI" as "[[%q SI] | DEAD]". *)
+  (*   2:{ iExFalso. simpl. iPoseProof (Lifetime.pending_not_shot with "LIVE DEAD") as "F". auto. } *)
+  (*   red_tl. iDestruct "SI" as "[%γu SI]". red_tl. iDestruct "SI" as "[%u SI]". *)
+  (*   red_tl. iDestruct "SI" as "[BQ [(PT & _ & WQ & P) | (_ & LIVE2 & _)]]". *)
+  (*   2:{ iPoseProof (Lifetime.pending_merge with "LIVE LIVE2") as "LIVE". *)
+  (*       iPoseProof (Lifetime.pending_wf with "LIVE") as "%S". exfalso. *)
+  (*       eapply Qp_add_lt_one. eauto. *)
+  (*   } *)
+  (*   iMod (Lifetime.pending_shot with "LIVE") as "#DEAD". iMod ("K" with "[DEAD]") as "_". *)
+  (*   { unfold spinlockInv. red_tl. iRight. eauto. } *)
+  (*   iPoseProof (make_isSpinlock n γ x P γk' k' L' l' LT' with "[PT BQ WQ P LO' PC']") as "ISL". *)
+  (*   { red_tl. iFrame. } *)
+  (*   rewrite red_syn_fupd. iMod "ISL". iModIntro. iFrame. auto. *)
+  (* Qed. *)
+
+  Lemma isSpinlock_get_data n x γx (S : sProp n) k L :
+    (⟦isSpinlock n x γx S k L, n⟧) -∗ (◆[k, L] ∗ ∃ N, (⌜↑N ⊆ E_Spinlock1⌝) ∗ inv n N (spinlockInv n x γx S)).
   Proof.
-    red_tl. simpl. iIntros "(ISL & LIVE & LO' & PC')". rewrite red_syn_fupd. red_tl.
-    iEval (unfold isSpinlock) in "ISL". red_tl.
-    iDestruct "ISL" as "[%N ISL]". iEval red_tl in "ISL".
-    iDestruct "ISL" as "(%IN & _ & %LT & SI)". rewrite red_syn_inv.
-    iInv "SI" as "SI" "K".
-    { unfold mask_has_Spinlock in MASK_SL. des_ifs. set_solver. }
-    simpl. iEval (unfold spinlockInv; red_tl) in "SI".
-    iDestruct "SI" as "[[%q SI] | DEAD]".
-    2:{ iExFalso. simpl. iPoseProof (Lifetime.pending_not_shot with "LIVE DEAD") as "F". auto. }
-    red_tl. iDestruct "SI" as "[%γu SI]". red_tl. iDestruct "SI" as "[%u SI]".
-    red_tl. iDestruct "SI" as "[BQ [(PT & _ & WQ & P) | (_ & LIVE2 & _)]]".
-    2:{ iPoseProof (Lifetime.pending_merge with "LIVE LIVE2") as "LIVE".
-        iPoseProof (Lifetime.pending_wf with "LIVE") as "%S". exfalso.
-        eapply Qp_add_lt_one. eauto.
-    }
-    iMod (Lifetime.pending_shot with "LIVE") as "#DEAD". iMod ("K" with "[DEAD]") as "_".
-    { unfold spinlockInv. red_tl. iRight. eauto. }
-    iPoseProof (make_isSpinlock n γ x P γk' k' L' l' LT' with "[PT BQ WQ P LO' PC']") as "ISL".
-    { red_tl. iFrame. }
-    rewrite red_syn_fupd. iMod "ISL". iModIntro. iFrame. auto.
+    iEval (unfold isSpinlock; red_tl). iIntros "[%N ISL]".
+    iEval (red_tl) in "ISL". iDestruct "ISL" as "[NS [LO INV]]". eauto.
   Qed.
 
   Lemma Spinlock_lock_spec
         tid n
-        (Es : coPsets)
-        (MASK_TOP : OwnEs_top Es)
-        (MASK_STTGT : mask_has_st_tgt Es n)
+        (E : coPset)
     :
-    ⊢ ∀ γ x (P : sProp n) γk k L l q (ds : list (nat * nat * sProp n)),
-        [@ tid, n, Es @]
-          ⧼⟦(((syn_tgt_interp_as n sndl (fun m => (➢ (scm_memory_black m))))
-                ∗ (⤉ isSpinlock n γ x P γk k L l)
-                ∗ ➢(live γk k q) ∗ (⤉ Duty(tid) ds)
-                ∗ ◇{List.map fst ds}(2 + L, 1))%S), 1+n⟧⧽
+    ⊢ ∀ x γx (S : sProp n) k L v (ds : list (nat * nat * sProp n)) (P R Q : sProp n),
+        [@ tid, n, E @]
+          ⧼(tgt_interp_as (state_tgt:=st_tgt_type) sndl (fun m => ((s_memory_black m) : sProp n)%S))
+             ∗ (⟦isSpinlock n x γx S k L, n⟧)
+             ∗ (⟦P, n⟧)
+             ∗ (⟦Duty(tid) ds, n⟧ ∗ ◇{List.map fst ds}(2 + L, 1))
+             ∗ (env_live_inv v (1+n) (⊤ ∖ E_Spinlock1) k
+                             (((x ↦ 1) ∗ (● γx 1))%S : sProp n)
+                             ((x ↦ 0) ∗ (● γx 0) ∗ S)%S
+               )
+             ∗ (⟦((● γx 0) ∗ R)%S, n⟧ =|1+n|={⊤ ∖ E_Spinlock1}=∗ ⟦((● γx 1) ∗ Q)%S, n⟧)
+             ∗ (□((⟦P, n⟧ ∗ ⟦Duty(tid) ds, n⟧) =|1+n|={E, ⊤}=∗ ⟦R, n⟧))
+             ∗ (□(⟦R, n⟧ =|1+n|={⊤, E}=∗ (⟦P, n⟧ ∗ ⟦Duty(tid) ds, n⟧)))
+          ⧽
             (OMod.close_itree Client (SCMem.mod gvs) (Spinlock.lock x))
-            ⧼rv, ⟦(∃ (γu u : τ{nat, 1+n}),
-                      (⤉ P) ∗ ➢(auexa_w γ (((q/2)%Qp, γu, u) : Qp * nat * nat)) ∗ ➢(live γk k (q/2))
-                       ∗ (⤉ Duty(tid) ((u, 0, ➢(@dead γu nat u)) :: ds)) ∗ ➢(@live γu nat u (1/2)) ∗ ◇[u](l, 1))%S, 1+n⟧⧽
+            ⧼rv, ⟦(S ∗ Q)%S, n⟧⧽
   .
   Proof.
-    iIntros (? ? ? ? ? ? ? ? ?).
+    iIntros (? ? ? ? ? ? ? ? ? ?).
     iStartTriple. iIntros "PRE POST". unfold Spinlock.lock.
-    (* Preprocess for induction. *)
-    iApply wpsim_free_all. auto.
-    unfold isSpinlock.
-    iEval (red_tl) in "PRE". iEval (rewrite red_syn_tgt_interp_as) in "PRE".
-    iDestruct "PRE" as "(#STINTP & (%N & SL) & LIVE & DUTY & PCS)".
-    iEval (red_tl; simpl) in "SL". iDestruct "SL" as "(%IN & #LO & %POS & INV)".
-    iEval (rewrite red_syn_inv) in "INV". iPoseProof "INV" as "#INV".
-    iMod (ccs_make k L _ 1 1 with "[PCS]") as "[CCS PCS]". iFrame. auto.
-    (* Set up induction hypothesis. *)
-    iMod (pcs_drop_le _ _ _ _ 1 with "PCS") as "PCS". lia. Unshelve. 2: lia.
-    iRevert "LIVE DUTY POST". iMod (ccs_ind2 with "CCS [] PCS") as "IND".
-    2:{ iApply "IND". }
-    iModIntro. iExists 0. iIntros "IH". iModIntro. simpl. iIntros "PCS LIVE DUTY POST".
-    (* Start an iteration. *)
+    (* Preprocess for induction: right after the call's yield. *)
     iEval (rewrite unfold_iter_eq). rred2r.
-    (* Number of Yield = 1. *)
-    iApply (wpsim_yieldR with "[DUTY PCS]").
-    2:{ iSplitL "DUTY". iApply "DUTY". iFrame. }
-    auto.
-    iIntros "DUTY FC". iModIntro. rred2r.
-    (* Case analysis on lock variable. *)
-    iInv "INV" as "SLI" "SLI_CLOSE". iEval (unfold spinlockInv; simpl; red_tl; simpl) in "SLI".
-    iDestruct "SLI" as "[[%q0 SLI] | DEAD]".
-    2:{ iExFalso. iPoseProof (Lifetime.pending_not_shot with "LIVE DEAD") as "%S". iFrame. auto. }
-    iEval (red_tl; simpl) in "SLI". iDestruct "SLI" as "[%γu0 SLI]".
-    iEval (red_tl; simpl) in "SLI". iDestruct "SLI" as "[%u0 SLI]".
-    iEval (red_tl; simpl) in "SLI". iDestruct "SLI" as "[qISB [ACQ|WAIT]]".
+    iDestruct "PRE" as "(#MEM & #ISL & P & [DUTY PCS] & #ELI & AU & #PUT_D & #GET_D)".
+    iMod (ccs_make _ _ _ 1 (100+v) with "[PCS]") as "[CCS PCS]".
+    { iFrame. iEval (unfold isSpinlock; red_tl) in "ISL". iDestruct "ISL" as "[%N ISL]".
+      iEval (red_tl) in "ISL". iDestruct "ISL" as "[_ [LO _]]". eauto.
+    }
+    iMod (pcs_drop_le _ _ _ _ 1 with "PCS") as "PCS".
+    lia.
+    iMod (pcs_decr _ _ 2 v with "PCS") as "[PCS PCS_ELI]".
+    lia.
+    iApply (wpsim_yieldR_gen2 with "[DUTY PCS]").
+    3:{ iFrame. }
+    lia.
+    lia.
+    iIntros "DUTY _ PCS".
+    iMod ("PUT_D" with "[P DUTY]") as "R".
+    { iFrame. }
+    iModIntro. rred2r.
+    (* Set up for ELI induction. *)
+    iEval (simpl) in "PCS".
+    iPoseProof (isSpinlock_get_data with "ISL") as "[_ (% & %NS & #INV_SL)]".
+    iInv "INV_SL" as "SL" "INV_SL_CLOSE". iEval (simpl) in "SL".
+    iEval (unfold spinlockInv; red_tl_all) in "SL".
+    iDestruct "SL" as "[%s SL]". iEval (red_tl_all) in "SL".
+    iDestruct "SL" as "(PTx & Lx & [(%UNLOCKED & S) | %LOCKED])"; cycle 1.
 
-    (** Case 1. Acquire the lock. *)
-    { iClear "IH". iDestruct "ACQ" as "(PT & PCk & qISW & PROP)".
-      iApply (SCMem_cas_fun_spec _ _ _ n with "[PT]"). auto.
-      { unfold mask_has_st_tgt. rewrite lookup_insert. pose mask_disjoint_spinlock_state_tgt. clear - d IN. set_solver. }
-      { iFrame. iApply tgt_interp_as_equiv. 2: iApply "STINTP".
-        iIntros. iEval (simpl; red_tl; simpl). iSplit; iIntros "P".
-        - iFrame. ss.
-        - iDestruct "P" as "[MB _]". iFrame.
+    { (* Do induction. *)
+      subst. iRevert "PCS INV_SL_CLOSE R AU POST".
+      iPoseProof (eli_ccs_ind with "[CCS PCS_ELI] [] [] [PTx Lx]") as "RES".
+      5:{ iSplitL; cycle 1. eauto. iEval (simpl; red_tl_all). iFrame. }
+      5:{ iIntros "PCS INV_SL_CLOSE R AU POST". iMod "RES".
+          iRevert "INV_SL_CLOSE R AU POST". iApply ("RES" with "PCS").
       }
-      iIntros (b) "(%u & %RES & PT)". destruct (SCMem.val_eq_dec 0 0).
-      2:{ exfalso. ss. }
-      clear e. des. subst. rred2r. iApply wpsim_tauR. rred2r.
-      (* Close the invariant spinlockInv: *)
-      (* 1. Allocate new obligation: I will release the lock. *)
-      iMod (alloc_obligation l 2) as "(%k1 & #LO1 & PC1)".
-      iMod (Lifetime.alloc k1) as "[%γk1 LIVE1]".
-      (* 2. Preprocess. *)
-      iPoseProof (Lifetime.pending_split _ (1/2)%Qp (1/2)%Qp with "[LIVE1]") as "[LIVE1 LIVE1']".
-      { iEval (rewrite Qp.half_half). iFrame. }
-      iEval (replace 2 with (1+1) by lia) in "PC1".
-      iPoseProof (pc_split with "PC1") as "[PC1 PC_POST]".
-      iMod (pc_mon _ 1 _ 1 _ _ with "PC1") as "PC1". Unshelve.
-      2:{ apply layer_drop_eq; auto. }
-      iMod (duty_add _ _ _ _ 0 ((➢ dead γk1 k1)%S : sProp n) with "[DUTY PC1] []") as "DUTY".
+      lia.
       { iFrame. }
-      { iModIntro. iEval (ss; red_tl). auto. }
-      iPoseProof (duty_tpromise with "DUTY") as "#PROM1".
-      { simpl. left. auto. }
-      iMod (link_new k1 k l 0 0 with "[PCk]") as "[#LINK1 _]".
-      { iFrame. eauto. }
-      iPoseProof ((Lifetime.pending_split _ (q/2)%Qp (q/2)%Qp) with "[LIVE]") as "[MYLIVE LIVE]".
-      { rewrite Qp.div_2. iFrame. }
-      iMod (auexa_b_w_update with "qISB qISW") as "[qISB qISW]".
-      (* Now close with SLI_CLOSE. *)
-      iMod ("SLI_CLOSE" with "[LIVE PT LIVE1' qISB]") as "_".
-      { iEval (unfold spinlockInv; simpl; red_tl; simpl).
-        iLeft. iExists (q/2)%Qp.
-        iEval (red_tl; simpl). iExists γk1. iEval (red_tl; simpl). iExists k1. iEval (red_tl; simpl).
-        iSplitL "qISB"; [iFrame|]. iRight. iFrame. auto.
+
+      - (* Inductive case. *)
+        iModIntro. iIntros "IH".
+        iIntros "A". iEval (simpl; red_tl_all) in "A". iDestruct "A" as "[PTx Lx]".
+        iModIntro. iIntros "PCS INV_SL_CLOSE R AU POST".
+        iApply (SCMem_cas_fun_spec with "[PTx] [-]").
+        3:{ iFrame. iApply (tgt_interp_as_equiv with "MEM"). ss. i.
+            red_tl_all. iSplit; [iIntros "A" | iIntros "[A M]"]; iFrame. ss.
+        }
+        lia.
+        { assert (↑N_Spinlock1 ## (↑N_state_tgt : coPset)).
+          { apply ndot_ne_disjoint. ss. }
+          set_solver.
+        }
+        iIntros (rv) "(% & %CASE & PTx)". destruct (SCMem.val_eq_dec 1 0).
+        { exfalso. ss. }
+        des; subst. rred2r. iApply wpsim_tauR. rred2r. iApply wpsim_tauR. rred2r.
+        iEval (rewrite unfold_iter_eq). rred2r.
+        iMod ("INV_SL_CLOSE" with "[PTx Lx]") as "_".
+        { iEval (simpl; unfold spinlockInv; red_tl_all). iExists 1. iEval red_tl_all.
+          iFrame. iRight. done.
+        }
+        iMod ("GET_D" with "R") as "[P DUTY]".
+        iApply (wpsim_yieldR_gen with "[DUTY PCS]").
+        2:{ iFrame. }
+        lia.
+        iIntros "DUTY FC". iMod ("PUT_D" with "[P DUTY]") as "R".
+        { iFrame. }
+        iModIntro. rred2r.
+        iInv "INV_SL" as "SL" "INV_SL_CLOSE".
+        iEval (simpl; unfold spinlockInv; red_tl_all) in "SL".
+        iDestruct "SL" as "[%s SL]". iEval (red_tl_all) in "SL".
+        iDestruct "SL" as "(PTx & Lx & [(%UNLOCKED & S) | %LOCKED])"; cycle 1.
+        { (* Finish with IH. *)
+          subst. iMod ("IH" with "FC [PTx Lx]") as "IH".
+          { iEval (simpl; red_tl_all). iFrame. }
+          iApply ("IH" with "INV_SL_CLOSE R AU POST").
+        }
+
+        (* Terminating case. *)
+        iClear "IH". subst.
+        iApply (SCMem_cas_fun_spec with "[PTx] [-]").
+        3:{ iFrame. iApply (tgt_interp_as_equiv with "MEM"). ss. i.
+            red_tl_all. iSplit; [iIntros "A" | iIntros "[A M]"]; iFrame. ss.
+        }
+        lia.
+        { assert (↑N_Spinlock1 ## (↑N_state_tgt : coPset)).
+          { apply ndot_ne_disjoint. ss. }
+          set_solver.
+        }
+        iIntros (rv) "(% & %CASE & PTx)". destruct (SCMem.val_eq_dec 0 0).
+        2:{ exfalso. ss. }
+        des; subst. rred2r. iApply wpsim_tauR. rred2r.
+        (* Post conditions. *)
+        iPoseProof ("AU" with "[Lx R]") as "AU".
+        { iEval red_tl_all. iFrame. }
+        iMod (FUpd_mask_mono _ _ _ (⊤ ∖ ↑N) with "AU") as "AU".
+        { set_solver. }
+        iEval (red_tl_all) in "AU". iDestruct "AU" as "[Lx Q]".
+        iMod ("INV_SL_CLOSE" with "[PTx Lx]") as "_".
+        { iEval (simpl; unfold spinlockInv; red_tl_all). iExists 1. iEval red_tl_all.
+          iFrame. iRight. done.
+        }
+        iApply "POST". iEval (red_tl). iFrame.
+
+      - (* Terminating case. *)
+        iIntros "T". iEval (simpl; red_tl_all) in "T". iDestruct "T" as "(PTx & Lx & S)".
+        iModIntro. iIntros "INV_SL_CLOSE R AU POST".
+        iApply (SCMem_cas_fun_spec with "[PTx] [-]").
+        3:{ iFrame. iApply (tgt_interp_as_equiv with "MEM"). ss. i.
+            red_tl_all. iSplit; [iIntros "A" | iIntros "[A M]"]; iFrame. ss.
+        }
+        lia.
+        { assert (↑N_Spinlock1 ## (↑N_state_tgt : coPset)).
+          { apply ndot_ne_disjoint. ss. }
+          set_solver.
+        }
+        iIntros (rv) "(% & %CASE & PTx)". destruct (SCMem.val_eq_dec 0 0).
+        2:{ exfalso. ss. }
+        des; subst. rred2r. iApply wpsim_tauR. rred2r.
+        (* Post conditions. *)
+        iPoseProof ("AU" with "[Lx R]") as "AU".
+        { iEval red_tl_all. iFrame. }
+        iMod (FUpd_mask_mono _ _ _ (⊤ ∖ ↑N) with "AU") as "AU".
+        { set_solver. }
+        iEval (red_tl_all) in "AU". iDestruct "AU" as "[Lx Q]".
+        iMod ("INV_SL_CLOSE" with "[PTx Lx]") as "_".
+        { iEval (simpl; unfold spinlockInv; red_tl_all). iExists 1. iEval red_tl_all.
+          iFrame. iRight. done.
+        }
+        iApply "POST". iEval (red_tl). iFrame.
+    }
+
+    { (* Terminating case. *)
+      subst.
+      iApply (SCMem_cas_fun_spec with "[PTx] [-]").
+      3:{ iFrame. iApply (tgt_interp_as_equiv with "MEM"). ss. i.
+          red_tl_all. iSplit; [iIntros "A" | iIntros "[A M]"]; iFrame. ss.
       }
-      (* Finish with POST. *)
-      iApply "POST". iEval (red_tl; simpl). iExists γk1. iEval (red_tl; simpl). iExists k1.
-      iEval (red_tl; simpl). iFrame.
-    }
-
-    (** Case 2. Miss the lock and loops. *)
-    { iDestruct "WAIT" as "(PT & LIVE_SL & LIVE_O & #OATH & #LINK)".
-      iApply (SCMem_cas_fun_spec _ _ _ n with "[PT]"). auto.
-      { unfold mask_has_st_tgt. rewrite lookup_insert. pose mask_disjoint_spinlock_state_tgt. clear - d IN. set_solver. }
-      { iFrame. iApply tgt_interp_as_equiv. 2: iApply "STINTP".
-        iIntros. iEval (simpl; red_tl; simpl). iSplit; iIntros "P".
-        - iFrame. ss.
-        - iDestruct "P" as "[MB _]". iFrame.
+      lia.
+      { assert (↑N_Spinlock1 ## (↑N_state_tgt : coPset)).
+        { apply ndot_ne_disjoint. ss. }
+        set_solver.
       }
-      iIntros (b) "(%u & %RES & PT)". destruct (SCMem.val_eq_dec 1 0).
-      { exfalso. ss. }
-      clear n0. des. subst. rred2r. iApply wpsim_tauR. rred2r. iApply wpsim_tauR.
-      (* Get credits from IH and the invariant. *)
-      iMod (tpromise_progress with "[FC]") as "[PC | DEAD]".
-      { iFrame. iApply "OATH". }
-      2:{ iExFalso. iPoseProof (Lifetime.pending_not_shot with "LIVE_O DEAD") as "%SALSE". auto. }
-      iMod (link_amplify with "[PC]") as "PC".
-      { iFrame. iApply "LINK". }
-      iMod ("IH" with "PC") as "IH".
-      (* Close the invariant spinlockInv. *)
-      iMod ("SLI_CLOSE" with "[qISB LIVE_SL LIVE_O PT]") as "_".
-      { iEval (unfold spinlockInv; simpl; red_tl; simpl).
-        iLeft. iExists q0. iEval (red_tl; simpl).
-        iExists γu0. iEval (red_tl; simpl). iExists u0. iEval (red_tl; simpl).
-        iSplitL "qISB"; [iFrame|]. iRight. iFrame. auto.
+      iIntros (rv) "(% & %CASE & PTx)". destruct (SCMem.val_eq_dec 0 0).
+      2:{ exfalso. ss. }
+      des; subst. rred2r. iApply wpsim_tauR. rred2r.
+      (* Post conditions. *)
+      iPoseProof ("AU" with "[Lx R]") as "AU".
+      { iEval red_tl_all. iFrame. }
+      iMod (FUpd_mask_mono _ _ _ (⊤ ∖ ↑N) with "AU") as "AU".
+      { set_solver. }
+      iEval (red_tl_all) in "AU". iDestruct "AU" as "[Lx Q]".
+      iMod ("INV_SL_CLOSE" with "[PTx Lx]") as "_".
+      { iEval (simpl; unfold spinlockInv; red_tl_all). iExists 1. iEval red_tl_all.
+        iFrame. iRight. done.
       }
-      (* Finish with IH. *)
-      iApply wpsim_stutter_mon. i; eauto. instantiate (1:=pt). i; auto.
-      iApply ("IH" with "LIVE DUTY POST").
+      iApply "POST". iEval (red_tl). iFrame.
     }
-  Qed.
+    Unshelve. lia.
 
-  Lemma red_syn_Spinlock_lock_spec
-        tid n
-        (Es : coPsets)
-    :
-    ⟦(∀ (γ : τ{nat})
-        (x : τ{SCMem.val})
-        (P : τ{Φ, 1+n})
-        (γk k L l : τ{nat})
-        (q : τ{Qp})
-        (ds : τ{ listT (nat * nat * Φ)%ftype, 1+n})
-       ,
-         [@ tid, n, Es @]
-           ⧼((syn_tgt_interp_as n sndl (fun m => (➢ (scm_memory_black m))))
-                ∗ (⤉ isSpinlock n γ x P γk k L l)
-                ∗ ➢(@live γk nat k q) ∗ (⤉ Duty(tid) ds)
-                ∗ ◇{List.map fst ds}(2 + L, 1))⧽
-             (OMod.close_itree Client (SCMem.mod gvs) (Spinlock.lock x))
-             ⧼rv, (∃ (γu u : τ{nat, 1+n}),
-                      (⤉ P) ∗ ➢(auexa_w γ (((q/2)%Qp, γu, u) : Qp * nat * nat)) ∗ ➢(@live γk nat k (q/2))
-                            ∗ (⤉ Duty(tid) ((u, 0, ➢(@dead γu nat u)) :: ds)) ∗ ➢(@live γu nat u (1/2)) ∗ ◇[u](l, 1))⧽)%S, 1+n⟧
-    =
-      (∀ γ x (P : sProp n) γk k L l q (ds : list (nat * nat * sProp n)),
-          [@ tid, n, Es @]
-            ⧼⟦((syn_tgt_interp_as n sndl (fun m => (➢ (scm_memory_black m))))
-                  ∗ (⤉ isSpinlock n γ x P γk k L l)
-                  ∗ ➢(live γk k q) ∗ (⤉ Duty(tid) ds)
-                  ∗ ◇{List.map fst ds}(2 + L, 1))%S, 1+n⟧⧽
-              (OMod.close_itree Client (SCMem.mod gvs) (Spinlock.lock x))
-              ⧼rv, ⟦(∃ (γu u : τ{nat, 1+n}),
-                        (⤉ P) ∗ ➢(auexa_w γ (((q/2)%Qp, γu, u) : Qp * nat * nat)) ∗ ➢(live γk k (q/2))
-                              ∗ (⤉ Duty(tid) ((u, 0, ➢(@dead γu nat u)) :: ds)) ∗ ➢(@live γu nat u (1/2)) ∗ ◇[u](l, 1))%S, 1+n⟧⧽)%I
-  .
-  Proof.
-    simpl.
-    red_tl. apply f_equal. extensionalities γ.
-    red_tl. apply f_equal. extensionalities x.
-    red_tl. apply f_equal. extensionalities P.
-    red_tl. apply f_equal. extensionalities γk.
-    red_tl. apply f_equal. extensionalities k.
-    red_tl. apply f_equal. extensionalities L.
-    red_tl. apply f_equal. extensionalities l.
-    red_tl. apply f_equal. extensionalities q.
-    red_tl. apply f_equal. extensionalities ds.
-    apply red_syn_non_atomic_triple.
-  Qed.
-
-  Lemma Spinlock_lock_syn_spec
-        tid n
-        (Es : coPsets)
-        (MASK_TOP : OwnEs_top Es)
-        (MASK_STTGT : mask_has_st_tgt Es n)
-    :
-    ⊢ ⟦(∀ (γ : τ{nat})
-          (x : τ{SCMem.val})
-          (P : τ{Φ, 1+n})
-          (γk k L l : τ{nat})
-          (q : τ{Qp})
-          (ds : τ{ listT (nat * nat * Φ)%ftype, 1+n})
-         ,
-           [@ tid, n, Es @]
-             ⧼((syn_tgt_interp_as n sndl (fun m => (➢ (scm_memory_black m))))
-                  ∗ (⤉ isSpinlock n γ x P γk k L l)
-                  ∗ ➢(@live γk nat k q) ∗ (⤉ Duty(tid) ds)
-                  ∗ ◇{List.map fst ds}(2 + L, 1))⧽
-               (OMod.close_itree Client (SCMem.mod gvs) (Spinlock.lock x))
-               ⧼rv, (∃ (γu u : τ{nat, 1+n}),
-                        (⤉ P) ∗ ➢(auexa_w γ (((q/2)%Qp, γu, u) : Qp * nat * nat)) ∗ ➢(@live γk nat k (q/2))
-                              ∗ (⤉ Duty(tid) ((u, 0, ➢(@dead γu nat u)) :: ds)) ∗ ➢(@live γu nat u (1/2)) ∗ ◇[u](l, 1))⧽)%S, 1+n⟧
-  .
-  Proof.
-    rewrite red_syn_Spinlock_lock_spec. iApply Spinlock_lock_spec. all: auto.
-  Qed.
-
-  Lemma Spinlock_unlock_spec
-        tid n
-        (Es : coPsets)
-        (MASK_TOP : OwnEs_top Es)
-        (MASK_STTGT : mask_has_st_tgt Es n)
-    :
-    ⊢ ∀ γ x (P : sProp n) γk k L l q (ds : list (nat * nat * sProp n)) γu u,
-        [@ tid, n, Es @]
-          ⧼⟦(((syn_tgt_interp_as n sndl (fun m => (➢ (scm_memory_black m))))
-                ∗ (⤉ isSpinlock n γ x P γk k L l) ∗ (⤉ P)
-                ∗ ➢(auexa_w γ (((q/2)%Qp, γu, u) : Qp * nat * nat)) ∗ ➢(live γk k (q/2))
-                ∗ (⤉ Duty(tid) ((u, 0, ➢(dead γu u)) :: ds)) ∗ ➢(live γu u (1/2))
-                ∗ ◇{List.map fst ((u, 0, ➢(dead γu u)) :: ds)}(1, 1)
-                ∗ ◇[k](1 + l, 1)))%S, 1+n⟧⧽
-            (OMod.close_itree Client (SCMem.mod gvs) (Spinlock.unlock x))
-            ⧼rv, ⟦((⤉ Duty(tid) ds) ∗ ➢(live γk k q))%S, 1+n⟧⧽
-  .
-  Proof.
-    iIntros (? ? ? ? ? ? ? ? ? ? ?).
-    iStartTriple. iIntros "PRE POST". unfold Spinlock.unlock.
-    (* Preprocess. *)
-    iApply wpsim_free_all. auto.
-    unfold isSpinlock. ss.
-    iEval (red_tl; simpl) in "PRE". iEval (rewrite red_syn_tgt_interp_as) in "PRE".
-    iDestruct "PRE" as "(#STINTP & (%N & SL) & P & WQ & LIVE & DUTY & LIVEU & PCS & PCk)".
-    iEval (red_tl; simpl) in "SL". iDestruct "SL" as "(%IN & #LO & %POS & INV)".
-    iEval (rewrite red_syn_inv) in "INV". iPoseProof "INV" as "#INV".
-    rred2r. iApply (wpsim_yieldR with "[DUTY PCS]").
-    2:{ iSplitL "DUTY". iFrame. iFrame. }
-    auto.
-    iIntros "DUTY FC". iModIntro.
-    (* Open invariant. *)
-    iInv "INV" as "SLI" "SLI_CLOSE". iEval (unfold spinlockInv; simpl; red_tl; simpl) in "SLI".
-    iDestruct "SLI" as "[[%q0 SLI] | DEAD]".
-    2:{ iExFalso. iPoseProof (Lifetime.pending_not_shot with "LIVE DEAD") as "%S". auto. }
-    iEval (red_tl; simpl) in "SLI". iDestruct "SLI" as "[%γu0 SLI]".
-    iEval (red_tl; simpl) in "SLI". iDestruct "SLI" as "[%u0 SLI]".
-    iEval (red_tl; simpl) in "SLI". iDestruct "SLI" as "[BQ [ACQ | WAIT]]".
-    { iExFalso. iDestruct "ACQ" as "(_ & _ & WQ2 & _)".
-      iPoseProof (auexa_w_w_false with "WQ WQ2") as "%S". inv F.
-    }
-    iDestruct "WAIT" as "(PT & LIVE2 & LIVEU2 & _)". rred2r.
-    (* Proceed simulation. *)
-    iApply (SCMem_store_fun_spec _ _ _ n with "[PT]"). auto.
-    { rewrite lookup_insert. pose mask_disjoint_spinlock_state_tgt. clear - d IN. set_solver. }
-    { iFrame. auto. }
-    iIntros (rv) "PT". rred2r. destruct rv. iApply wpsim_tauR. rred2r.
-    (* Close invariant. *)
-    iPoseProof (auexa_b_w_eq with "BQ WQ") as "%EQ". clarify.
-    iMod ("SLI_CLOSE" with "[P WQ PCk BQ PT]") as "_".
-    { simpl. iEval (unfold spinlockInv). red_tl. iLeft.
-      iExists (q/2)%Qp. red_tl. iExists γu. red_tl. iExists u.
-      red_tl. iSplitL "BQ". iFrame. iLeft. iFrame.
-    }
-    (* Postconditions. *)
-    iMod (Lifetime.pending_shot with "[LIVEU LIVEU2]") as "#DEADU".
-    { iEval (rewrite <- Qp.half_half). iApply (Lifetime.pending_merge with "LIVEU LIVEU2"). }
-    iMod (duty_fulfill with "[DUTY DEADU]") as "DUTY".
-    { iFrame. auto. }
-    iPoseProof (Lifetime.pending_merge with "LIVE LIVE2") as "LIVE".
-    iEval (rewrite Qp.div_2) in "LIVE". iApply "POST". red_tl. iFrame.
-  Qed.
-
-  Lemma red_syn_Spinlock_unlock_spec
-        tid n
-        (Es : coPsets)
-    :
-    ⟦(∀ (γ : τ{nat})
-        (x : τ{SCMem.val})
-        (P : τ{Φ, 1+n})
-        (γk k L l : τ{nat})
-        (q : τ{Qp})
-        (ds : τ{ listT (nat * nat * Φ)%ftype, 1+n})
-        (γu u : τ{nat, 1+n})
-       ,
-         [@ tid, n, Es @]
-           ⧼((syn_tgt_interp_as n sndl (fun m => (➢(scm_memory_black m))))
-               ∗ (⤉ isSpinlock n γ x P γk k L l) ∗ (⤉ P)
-               ∗ ➢(auexa_w γ (((q/2)%Qp, γu, u) : Qp * nat * nat)) ∗ ➢(@live γk nat k (q/2))
-               ∗ (⤉ Duty(tid) ((u, 0, ➢(@dead γu nat u)) :: ds)) ∗ ➢(@live γu nat u (1/2))
-               ∗ ◇{List.map fst ((u, 0, ➢(@dead γu nat u)) :: ds)}(1, 1)
-               ∗ ◇[k](1 + l, 1))⧽
-             (OMod.close_itree Client (SCMem.mod gvs) (Spinlock.unlock x))
-             ⧼rv, ((⤉ Duty(tid) ds) ∗ ➢(@live γk nat k q))⧽)%S, 1+n⟧
-    =
-      (∀ γ x (P : sProp n) γk k L l q (ds : list (nat * nat * sProp n)) γu u,
-          [@ tid, n, Es @]
-            ⧼⟦(((syn_tgt_interp_as n sndl (fun m => (➢ (scm_memory_black m))))
-                  ∗ (⤉ isSpinlock n γ x P γk k L l) ∗ (⤉ P)
-                  ∗ ➢(auexa_w γ (((q/2)%Qp, γu, u) : Qp * nat * nat)) ∗ ➢(live γk k (q/2))
-                  ∗ (⤉ Duty(tid) ((u, 0, ➢(dead γu u)) :: ds)) ∗ ➢(live γu u (1/2))
-                  ∗ ◇{List.map fst ((u, 0, ➢(dead γu u)) :: ds)}(1, 1)
-                  ∗ ◇[k](1 + l, 1)))%S, 1+n⟧⧽
-              (OMod.close_itree Client (SCMem.mod gvs) (Spinlock.unlock x))
-              ⧼rv, ⟦((⤉ Duty(tid) ds) ∗ ➢(live γk k q))%S, 1+n⟧⧽)%I
-  .
-  Proof.
-    red_tl. apply f_equal. extensionalities γ.
-    red_tl. apply f_equal. extensionalities x.
-    red_tl. apply f_equal. extensionalities P.
-    red_tl. apply f_equal. extensionalities γk.
-    red_tl. apply f_equal. extensionalities k.
-    red_tl. apply f_equal. extensionalities L.
-    red_tl. apply f_equal. extensionalities l.
-    red_tl. apply f_equal. extensionalities q.
-    red_tl. apply f_equal. extensionalities ds.
-    rewrite @red_tl_univ. apply f_equal. extensionalities γu.
-    rewrite @red_tl_univ. apply f_equal. extensionalities u.
-    apply red_syn_non_atomic_triple.
-  Qed.
-
-  Lemma Spinlock_unlock_syn_spec
-        tid n
-        (Es : coPsets)
-        (MASK_TOP : OwnEs_top Es)
-        (MASK_STTGT : mask_has_st_tgt Es n)
-    :
-    ⊢ ⟦(∀ (γ : τ{nat})
-          (x : τ{SCMem.val})
-          (P : τ{Φ, 1+n})
-          (γk k L l : τ{nat})
-          (q : τ{Qp})
-          (ds : τ{ listT (nat * nat * Φ)%ftype, 1+n})
-          (γu u : τ{nat, 1+n})
-         ,
-           [@ tid, n, Es @]
-             ⧼((syn_tgt_interp_as n sndl (fun m => (➢(scm_memory_black m))))
-                 ∗ (⤉ isSpinlock n γ x P γk k L l) ∗ (⤉ P)
-                 ∗ ➢(auexa_w γ (((q/2)%Qp, γu, u) : Qp * nat * nat)) ∗ ➢(@live γk nat k (q/2))
-                 ∗ (⤉ Duty(tid) ((u, 0, ➢(@dead γu nat u)) :: ds)) ∗ ➢(@live γu nat u (1/2))
-                 ∗ ◇{List.map fst ((u, 0, ➢(@dead γu nat u )) :: ds)}(1, 1)
-                 ∗ ◇[k](1 + l, 1))⧽
-               (OMod.close_itree Client (SCMem.mod gvs) (Spinlock.unlock x))
-               ⧼rv, ((⤉ Duty(tid) ds) ∗ ➢(@live γk nat k q))⧽)%S, 1+n⟧
-  .
-  Proof.
-    rewrite red_syn_Spinlock_unlock_spec. iApply Spinlock_unlock_spec. all: auto.
   Qed.
 
 End SPEC.
